Math/Algebra/C2_Groups/C2_2_morphism_theorems/theorems.lean
@@ -3,7 +3,7 @@ import Math.Algebra.C2_Groups.C2_2_morphism_theorems.definitions
 -- Theorem 2.2.1 (Homomorphism theorem)
 
 -- the quotient homomorphism is well-defined:
-theorem quotient_homomorphism_welldefined_lemma (G1 : Type u) (G2 : Type v)
+theorem quotient_homomorphism_welldefined_lemma (G1 G2 : Type)
 [MyGroup G1] [MyGroup G2] (φ : GroupHomomorphism G1 G2)
 (a b : left_coset' G1 (ker_to_normal_subgroup φ)) :
 a.carrier = b.carrier ->
@@ -42,7 +42,7 @@ a.carrier = b.carrier ->
 -- the quotient homomorphism is injective:
 -- here we can't use the standard definition of injective, because of the
 -- definition of left_coset'
-theorem quotient_homomorphism_injective_lemma (G1 : Type u) (G2 : Type v)
+theorem quotient_homomorphism_injective_lemma (G1 G2 : Type)
 [MyGroup G1] [MyGroup G2] (φ : GroupHomomorphism G1 G2) :
 quotient_is_injective (quotient_homomorphism φ) := by {
   rw [quotient_is_injective]
@@ -66,7 +66,7 @@ quotient_is_injective (quotient_homomorphism φ) := by {
 
 -- G/ker(φ) is isomorphic to im(φ)
 -- also here, the definition of G/H is a problem
-theorem quotient_isomorphism_lemma {G1 : Type u} {G2 : Type v}
+theorem quotient_isomorphism_lemma {G1 G2 : Type}
 [MyGroup G1] [MyGroup G2] (φ : GroupHomomorphism G1 G2) :
 quotient_is_isomorphic_to G1 (ker_to_normal_subgroup φ) (image_to_subgroup φ).carrier := by {
 
@@ -143,112 +143,7 @@ quotient_is_isomorphic_to G1 (ker_to_normal_subgroup φ) (image_to_subgroup φ).
 }
 
 
-/-
-theorem quotient_isomorphism_lemma {G1 : Type u} {G2 : Type v} {IM : Type v}
-[MyGroup G1] [MyGroup G2] [MyGroup IM] (φ : GroupHomomorphism G1 G2) (h_IM : im φ = IM) :
---quotient_is_isomorphic_to G1 (ker_to_normal_subgroup φ) (image_to_subgroup φ).carrier := by {
-quotient_is_isomorphic_to G1 (ker_to_normal_subgroup φ) IM := by {
---∃ ψ : quotient_isomorphism G1 (ker_to_normal_subgroup φ) (im φ), true := by {
-
-  let ψ2 : GroupHomomorphism (left_coset' G1 (ker_to_normal_subgroup φ)) G2 := quotient_homomorphism φ
-  have h : im ψ2 = im φ := by {
-    simp [ψ2]
-    rw [quotient_homomorphism]
-    simp [im]
-    ext x
-    constructor
-    simp
-    intro c h
-    obtain ⟨g_c, _⟩ := c
-    use g_c
-    simp
-    intros g h
-    let g_1 : left_coset' G1 (ker_to_normal_subgroup φ) := {
-      g := g
-      carrier := left_coset G1 (ker_to_normal_subgroup φ) g
-      h_carrier := by simp
-    }
-    use g_1
-  }
-
-  have h : IM = ↑(image_to_subgroup φ).carrier := by {
-    sorry
-  }
-  rw [h]
-
-  let ψ3 : GroupHomomorphism (left_coset' G1 (ker_to_normal_subgroup φ)) IM := {
-    f := λ x => by {
-      rw [← h_IM]
-      use ψ2.f x
-      rw [← h]
-      rw [im]
-      simp
-    }
-    mul := by {
-      simp
-      --intros a b
-      --simp [GroupHomomorphism.f, MyGroup.mul]
-      }
-      rw [h]
-
-      apply GroupHomomorphism.mul
-    }
-  }
-  let ψ4 : quotient_isomorphism G1 (ker_to_normal_subgroup φ) ↑(im φ) := {
-    toGroupHomomorphism := ψ3
-    injective' := by {
-      have : quotient_is_injective (quotient_homomorphism φ) := by {
-        apply quotient_homomorphism_injective_lemma
-      }
-      simp [ψ3, ψ2]
-      rw [quotient_is_injective]
-      rw [GroupHomomorphism.f]
-      simp
-      apply this
-    }
-    surjective := by {
-      rw [Function.Surjective]
-      simp
-      intros a h_a
-      rw [GroupHomomorphism.f]
-      simp [ψ3]
-      rw [GroupHomomorphism.f]
-      simp [ψ2, quotient_homomorphism]
-      simp [im] at h_a
-      obtain ⟨g_a, h_a⟩ := h_a
-      let a_1 : left_coset' G1 (ker_to_normal_subgroup φ) := {
-        g := g_a
-        carrier := left_coset G1 (ker_to_normal_subgroup φ) g_a
-        h_carrier := by simp
-      }
-      use a_1
-      rw [h_a]
-    }
-  }
-
-  let ψ5 : quotient_isomorphism G1 (ker_to_normal_subgroup φ) IM := {
-    toGroupHomomorphism := {
-      f := λ x => by {
-        rw [← h_IM]
-        use ψ3.f x
-        simp
-      }
-      mul := by {
-        intros a b
-
-      }
-    }
-    injective' := by {
-
-    }
-  }
-  rw [quotient_is_isomorphic_to]
-  use ψ5
-}
--/
-
-
-theorem cyclic_group_isomorphic_to_Z {G : Type u} [MyGroup G] (g : G)
+theorem cyclic_group_isomorphic_to_Z {G : Type} [MyGroup G] (g : G)
 (C : Subgroup G) (h_c : C = cyclic_group G g) :
 ∃ n : ℤ, quotient_is_isomorphic_to ℤ (nZ n) C.carrier := by {
 
@@ -309,8 +204,127 @@ theorem cyclic_group_isomorphic_to_Z {G : Type u} [MyGroup G] (g : G)
 }
 
 
+section isomorphism_theorem
+variable {G : Type} [MyGroup G] {H : Subgroup G} {N : normal_subgroup G}
 
-theorem isomorphism_theorem_1_i {G : Type u} [MyGroup G] (H : Subgroup G)
+-- i)
+-- HN := { h*n, h ∈ H, n ∈ N } is a subgroup of G
+def HN (H : Subgroup G) (N : normal_subgroup G) : Subgroup G := {
+  carrier := { x | ∃ h n : G, h ∈ H.carrier ∧ n ∈ N.carrier ∧ x = MyGroup.mul h n }
+  nonempty := by {
+    have : MyGroup.one ∈ { x | ∃ h n : G, h ∈ H.carrier ∧ n ∈ N.carrier ∧ x = MyGroup.mul h n } := by {
+      simp
+      use MyGroup.one
+      constructor
+      apply subgroup_contains_one_lemma
+      use MyGroup.one
+      constructor
+      apply subgroup_contains_one_lemma
+      rw [MyGroup.mul_one]
+    }
+    contrapose! this
+    rw [Set.eq_empty_iff_forall_not_mem] at this
+    apply this
+  }
+  mul_mem := by {
+    intros a b h
+    obtain ⟨h_a, h_b⟩ := h
+    simp at h_a h_b ⊢
+    obtain ⟨ha, h_ha, na, h_na, h_a⟩ := h_a
+    obtain ⟨hb, h_hb, nb, h_nb, h_b⟩ := h_b
+
+    -- use that N is normal
+    have h_normal : MyGroup.mul (MyGroup.mul (MyGroup.inv hb) na) hb ∈ N.carrier := by {
+      obtain ⟨N_SG, N_normal⟩ := N
+      rw [normal_iff_lemma] at N_normal
+      simp at h_na
+      specialize N_normal ⟨na, h_na⟩ hb
+      exact N_normal
+    }
+
+    use MyGroup.mul ha hb
+    constructor
+    apply Subgroup.mul_mem
+    exact ⟨h_ha, h_hb⟩
+    use MyGroup.mul (MyGroup.mul (MyGroup.mul (MyGroup.inv hb) na) hb) nb
+    constructor
+    apply Subgroup.mul_mem
+    exact ⟨h_normal, h_nb⟩
+    repeat rw [← MyGroup.mul_assoc]
+    nth_rewrite 4 [MyGroup.mul_assoc]
+    rw [MyGroup.mul_inv]
+    rw [MyGroup.mul_one]
+    rw [MyGroup.mul_assoc]
+    rw [h_a, h_b]
+  }
+  inv_mem := by {
+    intros a h_a
+    simp at h_a ⊢
+    obtain ⟨ha, h_ha, na, h_na, h_a⟩ := h_a
+
+    -- we use that N is normal again
+    have h_normal : MyGroup.mul (MyGroup.mul ha (MyGroup.inv na)) (MyGroup.inv ha) ∈ N.carrier := by {
+      have : MyGroup.mul (MyGroup.mul ha (MyGroup.inv na)) (MyGroup.inv ha) =
+            MyGroup.inv (MyGroup.mul (MyGroup.mul ha na) (MyGroup.inv ha)) := by {
+        repeat rw [mul_inv_lemma]
+        rw [double_inv_lemma]
+        repeat rw [MyGroup.mul_assoc]
+      }
+      rw [this]
+      apply Subgroup.inv_mem
+      obtain ⟨N_SG, N_normal⟩ := N
+      simp
+      rw [normal_iff_lemma] at N_normal
+      specialize N_normal ⟨na, h_na⟩ (MyGroup.inv ha)
+      simp at N_normal
+      rw [double_inv_lemma] at N_normal
+      exact N_normal
+    }
+    use (MyGroup.inv ha)
+    constructor
+    apply Subgroup.inv_mem
+    exact h_ha
+    use MyGroup.mul (MyGroup.mul ha (MyGroup.inv na)) (MyGroup.inv ha)
+    constructor
+    exact h_normal
+    repeat rw [← MyGroup.mul_assoc]
+    rw [MyGroup.inv_mul, MyGroup.one_mul]
+    rw [h_a]
+    rw [mul_inv_lemma]
+  }
+}
+
+
+-- ii) N is a normal Subgroup of HN
+def N' (H : Subgroup G) (N : normal_subgroup G) : normal_subgroup (HN H N).carrier := {
+  carrier := { x : ↑(HN H N).carrier | ∃ g : G, g = x ∧ g ∈ N.carrier }
+  nonempty := sorry
+  mul_mem := sorry
+  inv_mem := sorry
+  normal := sorry
+}
+
+
+-- ii) H ∩ N is a normal Subgroup of N
+def H_inter_N (H : Subgroup G) (N : normal_subgroup G) : normal_subgroup H.carrier := {
+  carrier := { h : H.carrier | ∃ g : G, h = g ∧ g ∈ N.carrier }
+  nonempty := sorry
+  mul_mem := sorry
+  inv_mem := sorry
+  normal := sorry
+}
+
+
+-- iii) H/(H ∩ N) ≅ HN/N
+theorem isomorphism_theorem_1 :
+quotient_is_isomorphic_to H.carrier (H_inter_N H N)
+(left_coset' (HN H N).carrier (N' H N)) := by {
+  -- we need a better way to use homomorphisms between quotient-groups.
+  sorry
+}
+
+/-
+theorem isomorphism_theorem1_i {G : Type} [MyGroup G] (H : Subgroup G)
 (N : normal_subgroup G) :
 ∃ S : Subgroup G, S.carrier =
 { x | ∃ h n : G, h ∈ H.carrier ∧ n ∈ N.carrier ∧ x = MyGroup.mul h n } := by {
@@ -323,9 +337,143 @@ theorem isomorphism_theorem_1_i {G : Type u} [MyGroup G] (H : Subgroup G)
     simp
     use MyGroup.one, MyGroup.one
     constructor
-
-
-
+    apply subgroup_contains_one_lemma
+    use MyGroup.one
+    constructor
+    apply subgroup_contains_one_lemma
+    rw [MyGroup.mul_one]
   }
+
+  -- a b ∈ HN -> a*b ∈ HN
+  have h_mul_mem : ∀ (a b : G), a ∈ HN ∧ b ∈ HN → MyGroup.mul a b ∈ HN := by {
+    intros a b h
+    obtain ⟨h_a, h_b⟩ := h
+    simp [HN] at h_a h_b ⊢
+    obtain ⟨ha, h_ha, na, h_na, h_a⟩ := h_a
+    obtain ⟨hb, h_hb, nb, h_nb, h_b⟩ := h_b
+
+    -- use that N is normal
+    have h_normal : MyGroup.mul (MyGroup.mul (MyGroup.inv hb) na) hb ∈ N.carrier := by {
+      obtain ⟨N_SG, N_normal⟩ := N
+      rw [normal_iff_lemma] at N_normal
+      simp at h_na
+      specialize N_normal ⟨na, h_na⟩ hb
+      exact N_normal
+    }
+
+    use MyGroup.mul ha hb
+    constructor
+    apply Subgroup.mul_mem
+    exact ⟨h_ha, h_hb⟩
+    use MyGroup.mul (MyGroup.mul (MyGroup.mul (MyGroup.inv hb) na) hb) nb
+    constructor
+    apply Subgroup.mul_mem
+    exact ⟨h_normal, h_nb⟩
+    repeat rw [← MyGroup.mul_assoc]
+    nth_rewrite 4 [MyGroup.mul_assoc]
+    rw [MyGroup.mul_inv]
+    rw [MyGroup.mul_one]
+    rw [MyGroup.mul_assoc]
+    rw [h_a, h_b]
+  }
+
+  -- a ∈ HN -> a⁻¹ ∈ HN
+  have h_inv_mem : ∀ a ∈ HN, MyGroup.inv a ∈ HN := by {
+    intros a h_a
+    simp [HN] at h_a ⊢
+    obtain ⟨ha, h_ha, na, h_na, h_a⟩ := h_a
+
+    -- we use that N is normal again
+    have h_normal : MyGroup.mul (MyGroup.mul ha (MyGroup.inv na)) (MyGroup.inv ha) ∈ N.carrier := by {
+      have : MyGroup.mul (MyGroup.mul ha (MyGroup.inv na)) (MyGroup.inv ha) =
+            MyGroup.inv (MyGroup.mul (MyGroup.mul ha na) (MyGroup.inv ha)) := by {
+        repeat rw [mul_inv_lemma]
+        rw [double_inv_lemma]
+        repeat rw [MyGroup.mul_assoc]
+      }
+      rw [this]
+      apply Subgroup.inv_mem
+      obtain ⟨N_SG, N_normal⟩ := N
+      simp
+      rw [normal_iff_lemma] at N_normal
+      specialize N_normal ⟨na, h_na⟩ (MyGroup.inv ha)
+      simp at N_normal
+      rw [double_inv_lemma] at N_normal
+      exact N_normal
+    }
+
+    use (MyGroup.inv ha)
+    constructor
+    apply Subgroup.inv_mem
+    exact h_ha
+    use MyGroup.mul (MyGroup.mul ha (MyGroup.inv na)) (MyGroup.inv ha)
+    constructor
+    exact h_normal
+    repeat rw [← MyGroup.mul_assoc]
+    rw [MyGroup.inv_mul, MyGroup.one_mul]
+    rw [h_a]
+    rw [mul_inv_lemma]
+  }
+
+  let S : Subgroup G := {
+    carrier := HN
+    nonempty := h_nonempty
+    mul_mem := h_mul_mem
+    inv_mem := h_inv_mem
+  }
+
+  use S
+}
+-/
+
+/-
+theorem isomorphism_theorem1_ii_1 {G : Type u} [MyGroup G] (H : Subgroup G)
+(N : normal_subgroup G) :
+∃ S : normal_subgroup H.carrier, S.carrier = H.carrier ∩ N.carrier := by {
   sorry
 }
+
+theorem isomorphism_theorem1_ii_2 {G : Type u} [MyGroup G] (H : Subgroup G)
+(N : normal_subgroup G) :
+∃ S : normal_subgroup G, S.carrier =
+-/
+
+/-
+def normal_subgroup_of_H_inter_N {G : Type} [MyGroup G] (H : Subgroup G) (N : normal_subgroup G) :
+SubgroupOfSubgroup H := {
+  carrier := { h : G | h ∈ N.carrier ∧ h ∈ H.carrier}
+
+  nonempty := by {
+    sorry
+  }
+  mul_mem := sorry
+  inv_mem := sorry
+  h_carrier := by simp
+}-/
+
+/-
+def normal_subgroup_of_H_inter_N {G : Type} [MyGroup G] {H : Subgroup G} {N : normal_subgroup G} :
+normal_subgroup H.carrier := {
+  carrier := by {
+    exact { h : H.carrier | ∃ g : G, g = h ∧ g ∈ N.carrier }
+  }
+  nonempty := by {
+    sorry
+  }
+  mul_mem := sorry
+  inv_mem := sorry
+  normal := sorry
+}
+
+--def exists_normal_subgroup_in_H {G : Type u} [MyGroup G] (H : Subgroup G) (N : normal_subgroup G) :
+--  ∃ H_N : normal_subgroup H.carrier, H_N.carrier = {h ∈ H.carrier | h ∈ N.carrier} :=
+
+theorem isomorphism_theorem1_iii {G : Type} [MyGroup G] (H : Subgroup G)
+(N : normal_subgroup G) :
+
+quotient_is_isomorphic_to H.carrier normal_subgroup_of_H_inter_N
+(left_coset' HN.carrier N )
+
+-/
+
+end isomorphism_theorem
